erasure/theories/ErasureFunction.v
@@ -8,7 +8,7 @@ From MetaCoq.PCUIC Require Import PCUICAst PCUICAstUtils
      PCUICCumulativity PCUICSR PCUICSafeLemmata
      PCUICValidity PCUICPrincipality PCUICElimination PCUICSN.
      
-From MetaCoq.SafeChecker Require Import PCUICSafeReduce PCUICSafeChecker PCUICSafeRetyping.
+From MetaCoq.SafeChecker Require Import PCUICErrors PCUICSafeReduce PCUICTypeChecker PCUICSafeRetyping.
 From MetaCoq.Erasure Require Import EAstUtils EArities Extract Prelim ErasureCorrectness EDeps.
 
 Local Open Scope string_scope.
