erasure/theories/Prelim.v
@@ -5,7 +5,7 @@ From MetaCoq.PCUIC Require Import PCUICTyping PCUICAst PCUICAstUtils
      PCUICSubstitution PCUICLiftSubst PCUICClosed
      PCUICWcbvEval PCUICSR  PCUICInversion PCUICGeneration
      PCUICContextConversion PCUICCanonicity.
-From MetaCoq.SafeChecker Require Import PCUICSafeReduce PCUICSafeChecker.
+From MetaCoq.SafeChecker Require Import PCUICErrors.
 From Coq Require Import Program ssreflect.
 
 
